Add Close to syntax of CC

theories/autosubst/CCAST.sig
@@ -7,6 +7,7 @@ cmode : Type
 cterm(cvar) : Type
 
 close : (bind cterm in cterm) -> cterm
+Close : (bind cterm in cterm) -> cterm
 
 cSort : cmode -> level -> cterm
 
